Migrate Constructor.v to new Points foundation

src/Constructor.v
@@ -1,69 +1,87 @@
 (** * A constructor for simple types *)
 
-Require Import ObAxioms.
-Require Import Lambda.
+Require Export Points.
+(*
 Require Import BohmTrees.
+*)
 
-Open Scope Lambda_scope.
-Open Scope Ob_scope.
+Section Exp.
+  Open Scope code_scope.
+  Variable Var : Set.
+  Let a := make_var Var 0.
+  Let b := make_var Var 1.
+  Let f := make_var Var 2.
+  Definition Exp := Eval compute in close (\a, \b, \f, b o f o a).
+End Exp.
+Notation "x --> y" := (Exp _ * x * y)%code : code_scope.
+Notation "x --> y" := ([Exp _] * x * y)%point : point_scope.
 
-Section pair.
-  Let x := VAR 0.
-  Let y := VAR 1.
-  Let z := VAR 2.
-  Definition pair := encode (\x,\y,\z, z * x * y).
-End pair.
-Notation "<< x , y >>" := (pair * x * y)%Ob : Ob_scope.
-Notation "<< x , y >>" := ([pair] * x * y)%Lambda : Lambda_scope.
-
-Definition is_pair (x : Ob) := x = <<x * K, x * F>>.
-Lemma pair_is_pair : forall x y, is_pair <<x, y>>.
+Lemma exp_i_i (Var : Set) : I --> I = (I : Point Var).
 Proof.
-  intros x y. compute. beta_reduce; auto.
+  unfold Exp; beta_eta.
 Qed.
 
-Definition sub_pair (x : Ob) := x [= <<TOP, TOP>>.
-Lemma sub_pair_pair : forall x y, sub_pair <<x, y>>.
+Section Pair.
+  Open Scope code_scope.
+  Variable Var : Set.
+  Let x := make_var Var 0.
+  Let y := make_var Var 1.
+  Let f := make_var Var 2.
+  Definition Pair := Eval compute in close (\x,\y,\f, f * x * y).
+End Pair.
+Notation "<< x , y >>" := (Pair _ * x * y)%code : code_scope.
+Notation "<< x , y >>" := ([Pair _] * x * y)%point : point_scope.
+
+Definition is_pair {Var : Set} (x : Point Var) := x = <<x * K, x * (K * I)>>.
+Lemma pair_is_pair (Var : Set) (x y : Point Var) : is_pair <<x, y>>.
 Proof.
-  intros x y. compute. beta_reduce.
-  apply LESS_trans with (C*(C*I*TOP)*y);
+  hnf; unfold Pair; beta_reduce; auto.
+Qed.
+
+Definition sub_pair {Var : Set} (x : Point Var) := x [= <<TOP, TOP>>.
+Lemma sub_pair_pair (Var : Set) (x y : Point Var) : sub_pair <<x, y>>.
+Proof.
+  unfold sub_pair; unfold Pair; eta_expand as f; beta_reduce.
   monotonicity; auto.
 Qed.
 
-Definition sub_pair_elim_intro : forall x, sub_pair x -> x [= <<x*K, x*F>>.
+Definition sub_pair_elim_intro {Var : Set} (x : Point Var) :
+  sub_pair x -> x [= <<x*K, x*(K*I)>>.
 Proof.
-  unfold sub_pair; unfold pair; compute.
-  intros x H.
-  eta_expand as y. beta_reduce.
-  eta_expand in H.
+  unfold sub_pair; unfold Pair; simpl.
+  intros H; eta_expand in H.
+  eta_expand as f; beta_reduce.
   (* TODO *)
 Admitted.
 
-Definition A := Join (<<s, r>> for s : Ob for r : Ob if r o s [= I).
-Notation "\\ x , y ; z" := ([A] * \x, \y, z)%Lambda
-  (at level 59, right associativity) : Lambda_scope.
+Definition A {Var : Set} :=
+  point_sup (<<s, r>> for s : Point Var for r : Point Var if r o s [= I).
+Notation "\\ x , y ; z" := (A * \x, \y, z)%code : code_scope.
+Notation "\\ x , y ; z" := (A * \x, \y, z)%point : point_scope.
 
 Section A_example.
-  Let a := VAR 0.
-  Let a' := VAR 1.
-  Let A_example := (\\a,a'; a --> a').
+  Variable Var : Set.
+  Let a := [make_var Var 0].
+  Let a' := [make_var Var 1].
+  Let A_example : Point Var := point_close (\\a,a'; a --> a').
 End A_example.
 
 Section raise.
-  Let x := VAR 3.
-  Let y := VAR 4.
+  Variable Var : Set.
+  Let x := [make_var Var 3].
+  Let y := [make_var Var 4].
 
-  Definition raise := encode (\x, \y, x).
-  Definition lower := encode (\x, x * [TOP]).
+  Definition raise := point_close (\x, \y, x).
+  Definition lower := point_close (\x, x * TOP).
 
-  Definition pull := encode (\x, \y, x || [div] * y).
-  Definition push := encode (\x, x * [BOT]).
+  Definition pull := point_close (\x, \y, x || [code_div] * y).
+  Definition push := point_close (\x, x * BOT).
 End raise.
 
-Lemma A_I_I : <<I, I>> [= A.
+Lemma A_I_I (Var : Set) : <<I, I>> [= (A : Point Var).
 Proof.
   unfold A.
-  assert (I o I [= I) as Heq; eta_expand; beta_reduce; auto.
+  assert (I o I [= (I : Point Var)) as Heq; eta_expand; beta_reduce; auto.
   (* TODO
   apply Join_ub_eq with (i := restrict2_intro _ I I Heq).
   *)
@@ -88,16 +106,17 @@ Qed.
 *)
 
 Section compose.
-  Let s := VAR 0.
-  Let a := VAR 1.
-  Let a' := VAR 2.
-  Let b := VAR 3.
-  Let b' := VAR 4.
+  Variable Var : Set.
+  Let s := [make_var Var 0].
+  Let a := [make_var Var 1].
+  Let a' := [make_var Var 2].
+  Let b := [make_var Var 3].
+  Let b' := [make_var Var 4].
 
-  Definition compose := encode
+  Definition compose := point_close
     (\s, s*\a,\a', s*\b,\b', <<a o b, b' o a'>>).
 
-  Definition conjugate := encode
+  Definition conjugate := point_close
     (\s, s*\a,\a', s*\b,\b', <<(a'-->b), (a-->b')>>).
 End compose.
 
@@ -111,7 +130,7 @@ Proof.
   unfold A_prop; split.
     compute; beta_reduce; auto.
   compute; eta_expand; beta_reduce.
-  apply LESS_trans with (a * F * (a * K * H));
+  apply LESS_trans with (a * (K*I) * (a * K * H));
     monotonicity; eta_expand in Hless; apply Hless.
 Qed.
 
@@ -124,45 +143,49 @@ Proof.
   unfold A_prop; split.
     compute; beta_reduce; auto.
   compute; eta_expand; eta_expand; beta_reduce.
-  apply LESS_trans with (a * F * (a * K * (H * H0)));
+  apply LESS_trans with (a * (K*I) * (a * K * (H * H0)));
     monotonicity; eta_expand in Hless; apply Hless.
 Qed.
 *)
 
-Definition A_def :=
+Definition A_def {Var : Set} : Point Var :=
   Y * ( K * <<I, I>>
-     || K * <<raise, lower>>
-     || K * <<pull, push>>
-     || compose
-     || conjugate).
+     || K * <<raise _, lower _>>
+     || K * <<pull _, push _>>
+     || compose _
+     || conjugate _).
 
-Lemma A_sound : A_def [= A.
+Lemma A_sound (Var : Set) : A_def [= (A : Point Var).
 Proof.
   (*
   unfold A.
   apply Join_lub.
   *)
   (* unfold A_prop; split. *)
+  (*
   unfold A_def.
   apply Y_lfp.
   intros y Hless.
   repeat (rewrite J_beta || rewrite K_beta).
   repeat apply J_lub.
+  *)
   (* TODO *)
 Admitted.
 
-Lemma A_complete : A [= A_def.
+Lemma A_complete (Var : Set) : (A : Point Var) [= A_def.
 Proof.
   unfold A.
+  (*
   apply Join_lub; unfold is_upper_bound.
   intros sr; induction sr as [[s r] Hless].
   apply LESS_conv.
   intros c Hdef Hconv.
   inversion Hconv.
+  *)
   (* TODO *)
 Admitted.
 
-Theorem A_definable : A = A_def.
+Theorem A_definable (Var : Set) : (A : Point Var) = A_def.
 Proof.
-  apply LESS_antisym ; apply A_sound || apply A_complete.
+  apply point_le_antisym ; apply A_sound || apply A_complete.
 Qed.
