src/ConstructorOld.v
@@ -1,0 +1,168 @@
+(** * A constructor for simple types *)
+
+Require Import ObAxioms.
+Require Import Lambda.
+Require Import BohmTrees.
+
+Open Scope Lambda_scope.
+Open Scope Ob_scope.
+
+Section pair.
+  Let x := VAR 0.
+  Let y := VAR 1.
+  Let z := VAR 2.
+  Definition pair := encode (\x,\y,\z, z * x * y).
+End pair.
+Notation "<< x , y >>" := (pair * x * y)%Ob : Ob_scope.
+Notation "<< x , y >>" := ([pair] * x * y)%Lambda : Lambda_scope.
+
+Definition is_pair (x : Ob) := x = <<x * K, x * F>>.
+Lemma pair_is_pair : forall x y, is_pair <<x, y>>.
+Proof.
+  intros x y. compute. beta_reduce; auto.
+Qed.
+
+Definition sub_pair (x : Ob) := x [= <<TOP, TOP>>.
+Lemma sub_pair_pair : forall x y, sub_pair <<x, y>>.
+Proof.
+  intros x y. compute. beta_reduce.
+  apply LESS_trans with (C*(C*I*TOP)*y);
+  monotonicity; auto.
+Qed.
+
+Definition sub_pair_elim_intro : forall x, sub_pair x -> x [= <<x*K, x*F>>.
+Proof.
+  unfold sub_pair; unfold pair; compute.
+  intros x H.
+  eta_expand as y. beta_reduce.
+  eta_expand in H.
+  (* TODO *)
+Admitted.
+
+Definition A := Join (<<s, r>> for s : Ob for r : Ob if r o s [= I).
+Notation "\\ x , y ; z" := ([A] * \x, \y, z)%Lambda
+  (at level 59, right associativity) : Lambda_scope.
+
+Section A_example.
+  Let a := VAR 0.
+  Let a' := VAR 1.
+  Let A_example := (\\a,a'; a --> a').
+End A_example.
+
+Section raise.
+  Let x := VAR 3.
+  Let y := VAR 4.
+
+  Definition raise := encode (\x, \y, x).
+  Definition lower := encode (\x, x * [TOP]).
+
+  Definition pull := encode (\x, \y, x || [div] * y).
+  Definition push := encode (\x, x * [BOT]).
+End raise.
+
+Lemma A_I_I : <<I, I>> [= A.
+Proof.
+  unfold A.
+  assert (I o I [= I) as Heq; eta_expand; beta_reduce; auto.
+  (* TODO
+  apply Join_ub_eq with (i := restrict2_intro _ I I Heq).
+  *)
+Admitted.
+
+(*
+Lemma A_raise_lower : A_prop <<raise, lower>>.
+Proof.
+  unfold A_prop; split;
+  [ apply pair_is_pair
+  | compute; eta_expand; beta_reduce; auto].
+Qed.
+
+Lemma A_pull_push : A_prop <<pull, push>>.
+Proof.
+  unfold A_prop; split.
+  apply pair_is_pair.
+  unfold pull.
+  freeze div in (compute; eta_expand; beta_reduce).
+  rewrite div_BOT; auto.
+Qed.
+*)
+
+Section compose.
+  Let s := VAR 0.
+  Let a := VAR 1.
+  Let a' := VAR 2.
+  Let b := VAR 3.
+  Let b' := VAR 4.
+
+  Definition compose := encode
+    (\s, s*\a,\a', s*\b,\b', <<a o b, b' o a'>>).
+
+  Definition conjugate := encode
+    (\s, s*\a,\a', s*\b,\b', <<(a'-->b), (a-->b')>>).
+End compose.
+
+(*
+Lemma A_compose : forall a, A_prop a -> A_prop (compose * a).
+Proof.
+  intros a H.
+  unfold A_prop in H; destruct H as [Hpair Hless].
+  unfold is_pair in Hpair.
+  rewrite Hpair.
+  unfold A_prop; split.
+    compute; beta_reduce; auto.
+  compute; eta_expand; beta_reduce.
+  apply LESS_trans with (a * F * (a * K * H));
+    monotonicity; eta_expand in Hless; apply Hless.
+Qed.
+
+Lemma A_conjugate : forall a, A_prop a -> A_prop (conjugate * a).
+Proof.
+  intros a H.
+  unfold A_prop in H; destruct H as [Hpair Hless].
+  unfold is_pair in Hpair.
+  rewrite Hpair.
+  unfold A_prop; split.
+    compute; beta_reduce; auto.
+  compute; eta_expand; eta_expand; beta_reduce.
+  apply LESS_trans with (a * F * (a * K * (H * H0)));
+    monotonicity; eta_expand in Hless; apply Hless.
+Qed.
+*)
+
+Definition A_def :=
+  Y * ( K * <<I, I>>
+     || K * <<raise, lower>>
+     || K * <<pull, push>>
+     || compose
+     || conjugate).
+
+Lemma A_sound : A_def [= A.
+Proof.
+  (*
+  unfold A.
+  apply Join_lub.
+  *)
+  (* unfold A_prop; split. *)
+  unfold A_def.
+  apply Y_lfp.
+  intros y Hless.
+  repeat (rewrite J_beta || rewrite K_beta).
+  repeat apply J_lub.
+  (* TODO *)
+Admitted.
+
+Lemma A_complete : A [= A_def.
+Proof.
+  unfold A.
+  apply Join_lub; unfold is_upper_bound.
+  intros sr; induction sr as [[s r] Hless].
+  apply LESS_conv.
+  intros c Hdef Hconv.
+  inversion Hconv.
+  (* TODO *)
+Admitted.
+
+Theorem A_definable : A = A_def.
+Proof.
+  apply LESS_antisym ; apply A_sound || apply A_complete.
+Qed.
