src/Notations.v
@@ -24,6 +24,7 @@ Reserved Notation "x [=] y" (at level 60, no associativity).
 Reserved Notation "x [!= y" (at level 60, no associativity).
 Reserved Notation "x ->> y" (at level 60, no associativity).
 Reserved Notation "\ x , y" (at level 58, right associativity).
+Reserved Notation "\\ x , y ; z" (at level 59, right associativity).
 
 Reserved Notation "[ x ]".
 
